c2itree/recog_site/recog_mod.v
@@ -1,0 +1,29 @@
+Require Import Any.
+Require Import ITreelib.
+Require Import ModSem.
+Require Import Skeleton.
+Require Import ConvC2ITree.
+From compcert Require Import AST Ctypes Clight Clightdefs Integers.
+
+Require amisc bmisc.
+
+
+Module amisc0.
+
+Import amisc.
+
+Let src_name := get_source_name Info.source_file.
+Definition prog := append_srcname prog src_name.
+Definition c_module := get_mod prog src_name.
+
+End amisc0. 
+
+Module bmisc0.
+
+Import bmisc.
+
+Let src_name := get_source_name Info.source_file.
+Definition prog := append_srcname prog src_name.
+Definition c_module := get_mod prog src_name.
+
+End bmisc0.
